composition/lww.fst
@@ -1,0 +1,132 @@
+module Lww
+open FStar.List.Tot
+
+open Library
+type s = (nat (*timestamp*) * nat (*value*))
+
+type op = nat (*value*)
+
+val get_id_s : s -> nat
+let get_id_s (t, v) = t
+val get_ele_s : s -> nat
+let get_ele_s (t, v) = v
+
+val app_op : s1:s -> op:(nat * op) -> Tot (s2:s {s2 = ((get_id op), (get_op op))})
+let app_op (t, v) (t1, v1) = (t1, v1)
+
+instance lww : datatype s op = {
+    Library.app_op = app_op
+  }
+
+val mem_ele : v:nat
+            -> l:list (nat * op)
+            -> Tot (b:bool{(exists id. mem (id, v) l) <==> b=true})
+let rec mem_ele n l =
+  match l with
+  |[] -> false
+  |(_, v)::xs -> (n = v) || mem_ele n xs
+
+val init : s
+let init = (0,0)
+
+val gt : l:list (nat * op)
+       -> init1:s
+       -> Pure s
+         (requires true)
+         (ensures (fun r -> (mem ((get_id_s r), (get_ele_s r)) l \/ r = init1) /\
+                         (forall e. mem e l ==> get_id_s r >= get_id e) /\ (get_id_s r >= get_id_s init1)))
+         (decreases (length l))
+#set-options "--z3rlimit 10000"
+let rec gt l init1 =
+  match l with
+  |[] -> init1
+  |(t, n)::xs -> if t > get_id_s init1 then (gt xs (t,n)) else (gt xs init1)
+
+val find : l:list (nat * op)
+         -> id:nat
+         -> Pure nat
+           (requires (unique l) /\ member id l /\ id > 0)
+           (ensures (fun v -> (mem (id, v) l) /\ mem_ele v l))
+let rec find l id =
+  match l with
+  |(id1, v)::xs -> if id = id1 then v else find xs id
+
+#set-options "--query_stats"
+val sim : tr:ae op
+        -> s1:s
+        -> Tot (b:bool {b = true <==> s1 = gt tr.l init} )
+let sim tr s1 = 
+  s1 = gt tr.l init
+
+val merge : ltr:ae op
+          -> l:s
+          -> atr:ae op
+          -> a:s 
+          -> btr:ae op
+          -> b:s 
+          -> Pure s (requires (forall e. mem e ltr.l ==> not (member (get_id e) atr.l)) /\
+                             (forall e. mem e atr.l ==> not (member (get_id e) btr.l)) /\
+                             (forall e. mem e ltr.l ==> not (member (get_id e) btr.l)) /\
+                             (sim ltr l /\ sim (union ltr atr) a /\ sim (union ltr btr) b) /\
+                             (forall e. mem e (absmerge ltr atr btr).l ==> get_id e > 0))
+                    (ensures (fun res -> ((get_id_s a >= get_id_s b) ==> res = a) /\
+                                      ((get_id_s b > get_id_s a) ==> res = b) /\
+                                      (get_id_s res >= get_id_s a /\ get_id_s res >= get_id_s b /\ get_id_s res >= get_id_s l) /\
+                                      (res = a \/ res = b)))
+#set-options "--z3rlimit 10000"
+let merge ltr l atr a btr b = 
+  assert ((get_id_s a = get_id_s b) ==> (get_id_s l = get_id_s a) /\ (get_id_s l = get_id_s b));
+  if (get_id_s a >= get_id_s b) then a else b
+
+val lemma : l:list (nat * op)
+          -> Lemma (requires unique l)
+                  (ensures (forall ele. member (get_id ele) l /\ (get_id ele > 0) ==> 
+                           (mem (get_id ele, (get_op ele)) l) ==> (get_op ele = find l (get_id ele))))
+                  (decreases (length l))
+let rec lemma l = 
+  match l with
+  |[] -> ()
+  |x::xs -> lemma xs 
+
+val prop_merge : ltr:ae op
+               -> l:s 
+               -> atr:ae op
+               -> a:s 
+               -> btr:ae op
+               -> b:s 
+               -> Lemma (requires (forall e. mem e ltr.l ==> not (member (get_id e) atr.l)) /\
+                                 (forall e. mem e atr.l ==> not (member (get_id e) btr.l)) /\
+                                 (forall e. mem e ltr.l ==> not (member (get_id e) btr.l)) /\
+                                 (sim ltr l /\ sim (union ltr atr) a /\ sim (union ltr btr) b)  /\
+                                 (forall e. mem e (absmerge ltr atr btr).l ==> get_id e > 0))
+                        (ensures (sim (absmerge ltr atr btr) (merge ltr l atr a btr b)))
+
+#set-options "--z3rlimit 10000000"
+let prop_merge ltr l atr a btr b = 
+  lemma (absmerge ltr atr btr).l;
+  ()
+
+val prop_oper : tr:ae op
+              -> st:s
+              -> op:(nat * op)
+              -> Lemma (requires (sim tr st) /\ 
+                                (not (member (get_id op) tr.l)) /\
+                                (get_id op > 0) /\
+                                (forall e. mem e tr.l ==> get_id e < get_id op))
+                      (ensures (sim (append tr op) (app_op st op)))
+let prop_oper tr st op = ()
+
+val convergence : tr:ae op
+                -> a:s
+                -> b:s  
+                -> Lemma (requires (sim tr a /\ sim tr b))
+                        (ensures a = b)
+let convergence tr a b = ()
+
+(*)instance _ : mrdt s op lww = {
+    Library.merge = merge;
+    Library.prop_merge = prop_merge;
+    Library.convergence = convergence;
+    Library.sim = sim;
+    Library.prop_oper = prop_oper
+ }*)
