composition/orset.fst
@@ -1,0 +1,223 @@
+module Orset
+open FStar.List.Tot
+
+open Library
+
+val member_s : id:nat 
+             -> l:list (nat * nat)
+             -> Tot (b:bool{(exists n. mem (id,n) l) <==> b=true})
+let rec member_s n l =
+    match l with
+    |[] -> false
+    |(id,_)::xs -> (n = id) || member_s n xs
+
+val unique_s : l:list (nat * nat)
+             -> Tot bool
+let rec unique_s l =
+    match l with
+    |[] -> true
+    |(id,_)::xs -> not (member_s id xs) && unique_s xs
+
+type s = l:list (nat (*unique id*) * nat (*element*)) {unique_s l}
+
+val filter_uni : f:((nat * nat) -> bool)
+               -> l:list (nat * nat) 
+               -> Lemma (requires (unique_s l))
+                       (ensures (unique_s (filter f l)))
+                               [SMTPat (filter f l)]
+
+#set-options "--z3rlimit 1000000"
+let rec filter_uni f l =
+  match l with
+  |[] -> ()
+  |x::xs -> filter_uni f xs
+
+type op =
+  |Add : nat (*element*) -> op
+  |Rem : nat (*element*) -> op
+
+val get_ele : op1:(nat * op) -> Tot (ele:nat {(exists id. op1 = (id, Add ele) \/ op1 = (id, Rem ele))})
+let get_ele op =
+  match op with
+  |(_, (Add ele)) -> ele
+  |(_, (Rem ele)) -> ele
+
+val opa : op1:(nat * op) -> Tot (b:bool {b = true <==> (exists id ele. op1 = (id, Add ele))})
+let opa op1 =
+  match op1 with
+  |(_, Add _) -> true
+  |_ -> false
+
+val opr : op1:(nat * op) -> Tot (b:bool {b = true <==> (exists id ele. op1 = (id, Rem ele))})
+let opr op1 = not (opa op1)
+
+val app_op : s1:s
+           -> op:(nat * op)
+           -> Pure s
+               (requires (not (member_s (get_id op) s1)))
+               (ensures (fun res -> (opa op ==> (forall e. mem e s1 \/ e = ((get_id op), (get_ele op)) <==> mem e res)) /\
+                                 (opr op ==> (forall e. mem e res <==> mem e s1 /\ snd e <> get_ele op))))
+let app_op s1 op1 =
+  match op1 with
+  |(id, Add ele) -> (id, ele)::s1
+  |(id, Rem ele) -> filter (fun e -> snd e <> ele) s1
+
+val filter_uni1 : f:((nat * op) -> bool)
+                -> l:list (nat * op) 
+                -> Lemma (requires (unique l))
+                        (ensures (unique (filter f l)))
+                           [SMTPat (filter f l)]
+let rec filter_uni1 f l = 
+  match l with
+  |[] -> ()
+  |x::xs -> filter_uni1 f xs
+
+(*)instance orset : datatype s op = {
+  Library.app_op = app_op
+}*)
+
+val except : #a:eqtype 
+             -> f:(a -> bool)
+             -> l:list a
+             -> Tot (l1:list a {forall e. mem e l1 <==> mem e l /\ not (f e)})
+let rec except #a f l =
+    match l with
+    |[] -> []
+    |hd::tl -> if not (f hd) then hd::(except f tl) else except f tl
+    
+#set-options "--query_stats"
+val sim : tr:ae op
+        -> s1:s 
+        -> Tot (b:bool {b = true <==> (forall a. mem a s1 <==> (mem ((fst a), Add (snd a)) tr.l /\
+                                   (forall r. mem r tr.l /\ fst a <> get_id r /\ opr r ==>
+                                         not (snd a = get_ele r && (tr.vis ((fst a), Add (snd a)) r)))))})
+let sim tr s1 =
+  let lsta = (filter (fun a -> opa a) tr.l) in
+  let lstr = (filter (fun r -> opr r) tr.l) in
+  let lst = except (fun a -> (existsb (fun r -> get_id a <> get_id r && get_ele r = get_ele a && tr.vis a r) lstr)) lsta in
+
+  forallb (fun e -> mem ((get_id e), (get_ele e)) s1) lst &&
+  forallb (fun e -> mem ((fst e), Add (snd e)) lst) s1
+
+val prop_oper : tr:ae op
+              -> st:s
+              -> op:(nat * op)
+              -> Lemma (requires (sim tr st) /\ (forall e. mem e tr.l ==> get_id e < get_id op) /\
+                                (not (member (get_id op) tr.l)))
+                      (ensures (sim (append tr op) (app_op st op)))
+
+#set-options "--z3rlimit 1000000"
+let prop_oper tr st op = ()
+
+val convergence : tr:ae op
+                -> a:s
+                -> b:s
+                -> Lemma (requires (sim tr a /\ sim tr b))
+                        (ensures (forall e. mem e a <==> mem e b))
+
+let convergence tr a b = ()
+
+val diff2 : a:list (nat * nat)
+          -> l:list (nat * nat)
+          -> Pure (list (nat * nat))
+            (requires (unique_s a /\ unique_s l))
+            (ensures (fun d -> (forall e. mem e d <==> mem e a /\ not (mem e l)) /\ unique_s d )) (decreases %[l;a;l;a])
+let diff2 a l = 
+  filter (fun e -> not (mem e l)) a
+
+val remove : l:s 
+           -> ele:(nat * nat)
+           -> Pure s 
+               (requires true)
+               (ensures (fun res -> (forall e. mem e res <==> mem e l /\ e <> ele)))
+let remove l ele =
+  filter (fun e -> e <> ele) l
+
+val merge1 : l:s
+           -> a:s 
+           -> b:s 
+           -> Pure s 
+           (requires (forall e. mem e (diff2 a l) ==> not (member_s (fst e) b)) /\
+                     (forall e. mem e (diff2 b l) ==> not (member_s (fst e) a)))
+           (ensures (fun res -> (forall e. mem e res <==> (mem e l /\ mem e a /\ mem e b) \/ 
+                             (mem e (diff2 a l)) \/ (mem e (diff2 b l)))))    (decreases %[l;a;b])
+#set-options "--z3rlimit 10000"
+let rec merge1 l a b = 
+  match l,a,b with
+  |[],[],[] -> []
+  |x::xs,_,_ -> if (mem x a && mem x b) then x::(merge1 xs (remove a x) (remove b x)) 
+                 else if (mem x a) then (merge1 xs (remove a x) b)
+                   else if (mem x b) then (merge1 xs a (remove b x))
+                     else (merge1 xs a b)
+  |[],x::xs,_ -> x::(merge1 [] xs b)
+  |[],[],x::xs -> b
+  
+val merge : ltr:ae op
+          -> l:s
+          -> atr:ae op
+          -> a:s
+          -> btr:ae op
+          -> b:s
+          -> Pure s (requires (forall e. mem e ltr.l ==> not (member (get_id e) atr.l)) /\
+                             (forall e. mem e atr.l ==> not (member (get_id e) btr.l)) /\
+                             (forall e. mem e ltr.l ==> not (member (get_id e) btr.l)) /\
+                             (sim ltr l /\ sim (union ltr atr) a /\ sim (union ltr btr) b))
+                   (ensures (fun res -> (forall e. mem e res <==> (mem e l /\ mem e a /\ mem e b) \/ 
+                                     (mem e (diff2 a l)) \/ (mem e (diff2 b l)))))
+
+#set-options "--z3rlimit 10000000"
+let merge ltr l atr a btr b = 
+    merge1 l a b
+
+val prop_merge : ltr:ae op
+               -> l:s
+               -> atr:ae op
+               -> a:s
+               -> btr:ae op
+               -> b:s
+               -> Lemma (requires (forall e. mem e ltr.l ==> not (member (get_id e) atr.l)) /\
+                                 (forall e. mem e atr.l ==> not (member (get_id e) btr.l)) /\
+                                 (forall e. mem e ltr.l ==> not (member (get_id e) btr.l)) /\
+                                 (sim ltr l /\ sim (union ltr atr) a /\ sim (union ltr btr) b))
+                       (ensures (sim (absmerge ltr atr btr) (merge ltr l atr a btr b)))
+
+#set-options "--z3rlimit 10000000"
+let prop_merge ltr l atr a btr b = 
+   assert (forall e. (mem e l /\ mem e a /\ mem e b) <==> (mem ((fst e), Add (snd e)) ltr.l /\ 
+           (forall r. mem r (absmerge ltr atr btr).l /\ fst e <> get_id r /\ opr r ==> 
+           not (snd e = get_ele r && (absmerge ltr atr btr).vis ((fst e), Add (snd e)) r))));
+
+    assert (forall e. (mem e (diff2 a l)) <==> (mem ((fst e), Add (snd e)) atr.l /\ (forall r. mem r atr.l /\ fst e <> get_id r /\
+           opr r ==> not (snd e = get_ele r && atr.vis ((fst e), Add (snd e)) r))));
+
+    assert (forall e. (mem e (diff2 b l)) <==> (mem ((fst e), Add (snd e)) btr.l /\ (forall r. mem r btr.l /\ fst e <> get_id r /\
+           opr r ==> not (snd e = get_ele r && btr.vis ((fst e), Add (snd e)) r))));
+
+    assert (forall e. (mem ((fst e), Add (snd e)) ltr.l /\ (forall r. mem r (absmerge ltr atr btr).l /\ fst e <> get_id r /\
+           opr r ==> not (snd e = get_ele r && (absmerge ltr atr btr).vis ((fst e), Add (snd e)) r))) \/ 
+           (mem ((fst e), Add (snd e)) atr.l /\ (forall r. mem r atr.l /\ fst e <> get_id r /\ 
+           opr r ==> not (snd e = get_ele r && atr.vis ((fst e), Add (snd e)) r))) \/
+           (mem ((fst e), Add (snd e)) btr.l /\ (forall r. mem r btr.l /\ fst e <> get_id r /\ 
+           opr r ==> not (snd e = get_ele r && btr.vis ((fst e), Add (snd e)) r))) <==>
+           (mem ((fst e), Add (snd e)) (absmerge ltr atr btr).l /\ (forall r. mem r (absmerge ltr atr btr).l /\ 
+           fst e <> get_id r /\ opr r ==> not (snd e = get_ele r && 
+           (absmerge ltr atr btr).vis ((fst e), Add (snd e)) r))));
+
+    assert (forall e. ((mem e l /\ mem e a /\ mem e b) \/ (mem e (diff2 a l)) \/ (mem e (diff2 b l))) <==> 
+           (mem ((fst e), Add (snd e)) (absmerge ltr atr btr).l /\ (forall r. mem r (absmerge ltr atr btr).l /\ 
+           fst e <> get_id r /\ opr r ==> not (snd e = get_ele r && 
+           (absmerge ltr atr btr).vis ((fst e), Add (snd e)) r))));
+
+    assert (forall e. (mem e (merge ltr l atr a btr b)) <==> 
+           (mem ((fst e), Add (snd e)) (absmerge ltr atr btr).l /\ (forall r. mem r (absmerge ltr atr btr).l /\ 
+           fst e <> get_id r /\ opr r ==> not (snd e = get_ele r && 
+           (absmerge ltr atr btr).vis ((fst e), Add (snd e)) r))));
+    ()
+
+(*)instance _ : mrdt s op orset = {
+  Library.merge = merge;
+  Library.prop_merge = prop_merge;
+  Library.convergence = convergence;
+  Library.sim = sim;
+  Library.prop_oper = prop_oper
+  }*)
